Improve the `insertLast` versions

RuleSystem/Rules/Wip.lean
@@ -5,50 +5,48 @@ namespace Instance
 def insertLast {n : ℕ} (inst : Instance (n + 1)) : Instance (n + 1)
   := ⟨inst.tags ∪ {Fin.last _}⟩
 
--- TODO: Can we use `insertLast` instead?
-def insertLast'' {n : ℕ} (rule : Rule n) (inst : rule.captureEmbed) : Instance (n + 1)
-  := ⟨inst.val.tags ∪ {Fin.last _}⟩
+def insertLastOnCaptureEmbed {n : ℕ} (rule : Rule n) (inst : rule.captureEmbed) : Instance (n + 1)
+  := insertLast inst
 
--- TODO: Finish proof
-theorem insertLast''_injective {n : ℕ} (rule : Rule n) : Function.Injective (insertLast'' rule) := by
-  sorry
+theorem insertLastOnCaptureEmbed_injective {n : ℕ} (rule : Rule n) : Function.Injective (insertLastOnCaptureEmbed rule) := by
+  intro x y insertLast_x_eq_insertLast_y
+  ext
+  apply eq_iff_tags_eq.mpr
+  ext tag
+  simp [insertLastOnCaptureEmbed, insertLast] at insertLast_x_eq_insertLast_y
+  constructor
+  -- TODO: Get rid of the symmetric case
+  · intro tag_mem_insertLast_x
+    cases Decidable.eq_or_ne tag (Fin.last _) with
+      | inl tag_eq_last =>
+        have := Instances.val_tags_CastPredPrecondition_of_notContainingLast x tag tag_mem_insertLast_x
+        contradiction
+      | inr tag_ne_last =>
+        have : tag ∈ y.val.tags ∪ {Fin.last _} := by
+          have := Finset.mem_union_left {Fin.last _} tag_mem_insertLast_x
+          rwa [insertLast_x_eq_insertLast_y] at this
+        simp [tag_ne_last] at this
+        assumption
+  · intro tag_mem_insertLast_y
+    cases Decidable.eq_or_ne tag (Fin.last _) with
+      | inl tag_eq_last =>
+        have := Instances.val_tags_CastPredPrecondition_of_notContainingLast y tag tag_mem_insertLast_y
+        contradiction
+      | inr tag_ne_last =>
+        have : tag ∈ x.val.tags ∪ {Fin.last _} := by
+          have := Finset.mem_union_left {Fin.last _} tag_mem_insertLast_y
+          rw [← insertLast_x_eq_insertLast_y] at this
+          assumption
+        simp [tag_ne_last] at this
+        assumption
 
-def insertLast''Embedding {n : ℕ} (rule : Rule n) : rule.captureEmbed ↪ Instance (n + 1)
-  := ⟨insertLast'' rule, insertLast''_injective rule⟩
+def insertLastOnCaptureEmbedEmbedding {n : ℕ} (rule : Rule n) : rule.captureEmbed ↪ Instance (n + 1)
+  := ⟨insertLastOnCaptureEmbed rule, insertLastOnCaptureEmbed_injective rule⟩
 end Instance
 
 namespace Rule
 
 def captureEmbedInsertLast {n : ℕ} (rule : Rule n) : Instances (n + 1)
-  := rule.captureEmbed.attach.map (Instance.insertLast''Embedding rule)
-
--- def captureEmbedEmbedding
-
--- instance {n : ℕ} (rule : Rule n) : CoeDep (Instances (n + 1)) rule.captureEmbed (Finset (@Instances.notContainingLast n)) where
---   coe := by
---     exists rule.captureEmbed.map (Subtype (· ∈ @Instances.notContainingLast n))
-
---     sorry
-
-
--- TODO: Finish this 🍊
--- (Instances.insertLast' rule.val.captureEmbed)
--- application type mismatch
---   Instances.insertLast' (↑rule).captureEmbed
--- argument
---   (↑rule).captureEmbed
--- has type
---   Instances (n + 1) : Type
--- but is expected to have type
---   Finset { x // x ∈ Instances.notContainingLast } : Type
-
--- This is probably wrong / not what we want
--- instance CoeDepCaptureEmbedNotContainingLast {n : ℕ} (rule : Rule n) (x : Instances (n + 1)) (h : x = rule.captureEmbed)
---   : CoeDep (Instances (n + 1)) x (Finset (@Instances.notContainingLast n)) where
---     coe := by
---       exists x.val
-
---       -- exists rule.captureEmbed
---       sorry
+  := rule.captureEmbed.attach.map (Instance.insertLastOnCaptureEmbedEmbedding rule)
 
 end Rule
