RuleSystem.lean
@@ -1,8 +1,11 @@
 -- This module serves as the root of the `RuleSystem` library.
 -- Import modules here that should be built as part of the library.
+
+-- TODO: Better method to import everything
 import RuleSystem.Rules.Theorems.Basic
 import RuleSystem.Rules.Theorems.Advanced
 import RuleSystem.Rules.Theorems.Wip
 import RuleSystem.Rules.Theorems.Embeddings.All
 import RuleSystem.Rules.Theorems.Embeddings.Positive
+import RuleSystem.Rules.Theorems.Embeddings.PositiveWip
 import RuleSystem.Rules.Theorems.Embeddings.Negative
